src/Source_Properties.v
@@ -2,23 +2,25 @@
 
 Require Import Source_Definitions Core_Infrastructure.
 
-Theorem s_typing_implies_s_ok : forall G e s,
-  s_typing G e s -> s_ok G.
-Proof. (* TODO *)
-  intros G e s P.
-  induction P; auto.
-  unfolds s_ok.
-  split.
-  pick_fresh x.
+Lemma s_type_extract : forall (s : typ_satisfying s_type),
+  s_type (obj s).
+Proof. intro. destruct* s. Qed.
+Hint Resolve s_type_extract.
 
-Admitted. 
+Theorem s_typing_implies_ok : forall G e s,
+  s_typing G e s -> ok G.
+Proof.
+  induction 1; auto.
+  (* TODO write a tactic that makes this line cleaner *)
+  pick_fresh x. assert (ok (G & x ~ s1)); auto.
+Qed.
 
 Theorem s_typing_implies_s_type : forall G e s,
-  s_typing G e s -> s_type s.
-Proof. (* TODO *)
-Admitted. 
+  s_typing G e s -> s_type (obj s).
+Proof. auto. Qed.
 
 Theorem s_typing_implies_s_term : forall G e s,
   s_typing G e s -> s_term e.
-Proof. (* TODO *)
-Admitted. 
+Proof.
+  induction 1; eauto.
+Qed.
